src/dvspec/dafny/att_spec_proofs/ind_inv.dfy
@@ -5,61 +5,82 @@ include "../specification/network.dfy"
 include "../specification/dvn.dfy"
 include "../att_spec_proofs/inv.dfy"
 
-module AttInductiveInvariants
+module Att_Ind_Inv_With_Empty_Initial_Attestation_Slashing_DB
 {
     import opened Types 
     import opened CommonFunctions
     import opened ConsensusSpec
     import opened NetworkSpec
     import opened DVCNode_Spec
-    import opened DV
-    import opened AttInvariants
+    import opened DV    
+    import opened Att_Inv_With_Empty_Initial_Attestation_Slashing_DB
 
-    predicate att_ind_inv<D(!new, 0)>(dvn: DVState)
-    {
-        && forall i: Slot :: no_conflict_decisions_pred1_in_sec_3_1(dvn.consensus_on_attestation_data[i])
-        && forall i: Slot :: no_decisions_pred2_in_sec_3_1(dvn.consensus_on_attestation_data[i])
-        && consistant_att_slashing_databases_between_honest_nodes_pred3_in_sec_3_2<D>(dvn)
-        && consistant_attestations_in_one_slashing_db_pred4_in_sec_3_2<D>(dvn)
-        && curr_att_duty_is_last_served_duty_pred5_in_sec_3_3<D>(dvn)       
-        && exisiting_consensus_instance_for_curr_att_duty_pred6_in_sec_3_3<D>(dvn)       
-        && active_consensus_instances_imples_existence_of_curr_att_duty_pred7_in_sec_3_3<D>(dvn)       
-        && queued_duties_later_than_curr_att_duty_pred8_in_sec_3_3<D>(dvn)       
-        && submitted_att_by_curr_att_duty_pred9_in_sec_3_3<D>(dvn)       
-        && none_latest_att_duty_implies_empty_att_duty_queue_pred10_in_sec_3_4<D>(dvn)       
-        && queued_duties_later_than_latest_att_duty_pred11_in_sec_3_4<D>(dvn)       
-        && submitted_att_by_latest_att_duty_pred12_in_sec_3_4<D>(dvn)       
-        && active_consensus_instances_for_slots_until_latest_att_duty_pred13_in_sec_3_4<D>(dvn)       
-        && no_active_consensus_instances_for_queued_att_duties_pred14_in_sec_3_5<D>(dvn)       
-        && att_from_imported_block_is_decided_value_pred16_in_sec_3_6<D>(dvn)       
-        && old_duty_has_submitted_att_data_pred17_in_sec_3_6<D>(dvn)       
-        && AttConsensusDecided_is_decided_value_pred18_in_sec_3_7<D>(dvn)       
-        && local_active_consensus_instance_not_later_than_latest_duty_pred19a_in_sec_3_7<D>(dvn)       
-        && no_latest_duty_is_older_than_distributed_undecided_consensus_instance_pred19b_in_sec_3_7<D>(dvn)       
-        && strictly_monotonic_att_duties_queue_pred20_in_sec_3_7<D>(dvn)       
-        && constructable_set_of_att_shares_has_at_least_one_share_from_honest_node_pred21_in_sec_3_7<D>(dvn)       
-        && no_missing_att_in_db_pred22_in_sec_3_7<D>(dvn)       
-        && no_missing_att_in_db_pred23_in_sec_3_7<D>(dvn)       
-        && pred24<D>(dvn)
-        && pred25_in_sec_3_7<D>(dvn)  
-        && sent_att_share_from_honest_node_pred26_in_sec_3_7<D>(dvn)       
-        && undecided_dist_consensus_instance_implies_latest_att_duty_pred27_in_sec_3_7<D>(dvn)       
-        && at_most_one_undecided_dist_consensus_instance_pred28_in_sec_3_7<D>(dvn)       
-        && shared_rcvd_att_duties_pred29_in_sec_3_7<D>(dvn)      
-        && same_function_to_reconstruct_attestations_pred30_in_sec_3_7<D>(dvn) 
+    lemma ConsensusSpec_Init_implies_inv41<D(!new, 0)>(dvn: DVState, ci: ConsensusInstance<D>)
+    requires ConsensusSpec.Init(ci, dvn.all_nodes, dvn.honest_nodes_states.Keys)
+    ensures inv41(ci)
+    { } 
+
+    lemma NextConsensusDecides_implies_inv41<D(!new, 0)>(
+            s: ConsensusInstance,
+            honest_nodes_validity_predicates: map<BLSPubkey, D -> bool>,        
+            s': ConsensusInstance
+        )
+    requires inv41(s) && isConditionForSafetyTrue(s)
+    requires ConsensusSpec.NextConsensusDecides(s, honest_nodes_validity_predicates, s')
+    ensures inv41(s')
+    { } 
+
+    lemma ConsensusSpec_Next_implies_inv41<D(!new, 0)>(
+            s: ConsensusInstance,
+            honest_nodes_validity_predicates: map<BLSPubkey, D -> bool>,        
+            s': ConsensusInstance,
+            output: Optional<OutCommand>
+        )
+    requires inv41(s) && isConditionForSafetyTrue(s)
+    requires ConsensusSpec.Next(s, honest_nodes_validity_predicates, s', output)
+    ensures inv41(s')
+    { 
+        assert NextConsensusDecides(s, honest_nodes_validity_predicates, s');
+        NextConsensusDecides_implies_inv41(s, honest_nodes_validity_predicates, s');
+        assert inv41(s');
+        assert NextNodeStep(s', honest_nodes_validity_predicates, output);
+        assert inv41(s');
     }
+
+    lemma DV_Init_implies_inv41(dvn: DVState)
+    requires DV.Init(dvn, {}) 
+    ensures forall s: Slot :: inv41(dvn.consensus_on_attestation_data[s])
+    { } 
+
+    // TODO: Remove {:axiom} and prove this lemma later.
+    lemma {:axiom} DV_Next_implies_inv41(dvn: DVState, dvn': DVState)
+    requires forall s: Slot :: inv41(dvn.consensus_on_attestation_data[s])
+    requires exists event: DV.Event :: DV.NextEvent(dvn, event, dvn')
+    ensures forall s: Slot :: inv41(dvn'.consensus_on_attestation_data[s])
+   
+    lemma a_valid_decided_value_has_at_least_f_plus_1_honest_nodes(s: ConsensusInstance<AttestationData>)
+    requires is_a_valid_decided_value(s)
+    ensures exists h_nodes |
+                && h_nodes <= s.honest_nodes_validity_functions.Keys  
+                && |h_nodes| >= quorum(|s.all_nodes|) - (|s.all_nodes| - |s.honest_nodes_status.Keys|)
+                ::
+                honest_nodes_with_validityPredicate(s, h_nodes)
+    {}
+
+
+    lemma DV_Init_implies_inv42(dvn: DVState)
+    requires DV.Init(dvn, {}) 
+    ensures inv42(dvn)
+    { } 
+
+    // TODO: Remove {:axiom} and prove this lemma later.
+    lemma {:axiom} DV_Next_implies_inv42(dvn: DVState, dvn': DVState)
+    requires inv42(dvn)
+    requires exists event: DV.Event :: DV.NextEvent(dvn, event, dvn')
+    ensures inv42(dvn')
+
     
-
-
-
-/*
-    predicate fixed_set_all_nodes_in_sec_3_7<D(!new, 0)>(
-        s: DVCNodeState, 
-        e: Types.Event,
-        s': DVCNodeState)
-    requires f_process_event.requires(s, e)
-    {
-        s' == DVCNode_Spec.f_process_event(s, e).state ==> s.peers == s'.peers                
-    }
-    */
+    lemma DV_Init_implies_thresholds(dvn: DVState)
+    requires DV.Init(dvn, {})
+    ensures |dvn.honest_nodes_states.Keys| >= |dvn.all_nodes| - f(|dvn.all_nodes|) 
 }
