src/dvspec/dafny/specification/consensus.dfy
@@ -101,7 +101,9 @@ module ConsensusSpec
             exists h_nodes |
                 && h_nodes <= s.honest_nodes_validity_functions.Keys  
                 // && |h_nodes| >= f(|s.all_nodes|) + 1
-                && |h_nodes| >= quorum(|s.all_nodes|) - f(|s.all_nodes|) 
+                // && |h_nodes| >= quorum(|s.all_nodes|) - f(|s.all_nodes|) 
+                && |h_nodes| >= quorum(|s.all_nodes|) 
+                                        - (|s.all_nodes| - |s.honest_nodes_status.Keys|)
                 ::
                 forall n | n in h_nodes :: 
                     exists vp: D -> bool | vp in s.honest_nodes_validity_functions[n] :: vp(s.decided_value.safe_get())       
